Labeled/FSets/Substitution.v
@@ -1,7 +1,7 @@
-Require Export LSyntax.
+Add LoadPath "../..".
+Require Export Syntax.
 Require Import Arith.
 Require Import LibList.
-
 Require Import LibTactics. (* case_if *)
 
 (* Term variable substitution *)
@@ -15,14 +15,13 @@ match N with
 | box_L N' => box_L [M//x]N'
 | unbox_L N' => unbox_L [M//x]N'
 | get_L w N' => get_L w [M//x]N'
-| letd_L N' N'' => letd_L [M//x]N' [M//S x]N''
+| letdia_L N' N'' => letdia_L [M//x]N' [M//S x]N''
 | here_L N' => here_L [M//x]N'
 | fetch_L w N' => fetch_L w [M//x]N'
 end
 where " [ M // x ] N " := (subst_t M x N) : labeled_is5_scope.
 
 Open Scope labeled_is5_scope.
-
 
 (* Substitute L[0] for n, L[1] for n+1,.. in M *)
 Fixpoint subst_list L n N :=
@@ -39,20 +38,11 @@ match N with
 | hyp_L v => hyp_L v
 | lam_L t N' => lam_L t {{w1//w2}}N'
 | appl_L N' N'' => appl_L {{w1//w2}}N' {{w1//w2}}N''
-| box_L N' => match w1, w2 with
-              | fwo w1', bwo w2' => box_L {{w1 // bwo (S w2')}}N'
-              | fwo w1', fwo w2' => box_L {{w1 // w2}} N'
-              | bwo w1', bwo w2' => box_L {{bwo (S w1') // bwo (S w2')}} N'
-              | bwo w1', fwo w2' => box_L {{bwo (S w1')//w2}} N'
-            end
+| box_L N' => box_L {{shift_vwo w1 // shift_vwo w2}} N'
 | unbox_L N' => unbox_L {{w1//w2}}N'
 | get_L w N' => get_L (if eq_vwo_dec w w2 then w1 else w) {{w1//w2}}N'
-| letd_L N' N'' => match w1, w2 with
-                   | fwo w1', bwo w2' => letd_L {{w1 // w2}}N' {{w1 // bwo (S w2')}}N''
-                   | fwo w1', fwo w2' => letd_L {{w1 // w2}}N' {{w1 // w2}}N''
-                   | bwo w1', bwo w2' => letd_L {{w1//w2}}N' {{bwo (S w1') // bwo (S w2')}} N''
-                   | bwo w1', fwo w2' => letd_L {{w1//w2}}N' {{bwo (S w1')//w2}}N''
-                 end
+| letdia_L N' N'' =>
+  letdia_L {{w1 // w2}} N' {{shift_vwo w1 // shift_vwo w2}} N''
 | here_L N' => here_L {{w1//w2}}N'
 | fetch_L w N' => fetch_L (if eq_vwo_dec w w2 then w1 else w) {{w1//w2}}N'
 end
@@ -64,7 +54,7 @@ Notation " M ^ w " := (open_w M w) : labeled_is5_scope.
 Section Substitution_lemmas.
 
 Lemma no_unbound_worlds_subst_w_id:
-forall M w n 
+forall M w n
   (H_unbound: unbound_worlds n M = nil),
   {{w//bwo n}}M = M.
 intros;
@@ -76,14 +66,12 @@ try (rewrite IHM); try auto.
 apply app_eq_nil in H_unbound;
 destruct H_unbound;
 rewrite IHM1; try rewrite IHM2; auto.
-(* box *)
-destruct w; try rewrite IHM; auto.
 (* get *)
 destruct (eq_vwo_dec v (bwo n));
 [ subst; discriminate | reflexivity ];
 try (destruct v; [discriminate | assumption]).
 destruct v; [discriminate | assumption].
-(* letd *)
+(* letdia *)
 destruct w;
 inversion H_unbound; auto;
 apply app_eq_nil in H_unbound;
@@ -96,51 +84,49 @@ try (destruct w; [discriminate | assumption]).
 destruct v; [discriminate | assumption].
 Qed.
 
-
 Lemma closed_w_subst_id:
-forall M w n 
+forall M w n
   (HT: lc_w_n M n),
   {{w//bwo n}} M = M.
-intros.
-apply no_unbound_worlds_subst_w_id.
-apply closed_no_unbound_worlds.
+intros;
+apply no_unbound_worlds_subst_w_id;
+apply closed_no_unbound_worlds;
 assumption.
 Qed.
 
 Lemma subst_order_irrelevant:
-forall N M n m w 
+forall N M n m w
   (H_LC: lc_w M),
   {{w//bwo m}}([M//n]N) = [M//n]({{w//bwo m}}N).
 unfold open_w; intro;
 induction N; intros; simpl; try (rewrite IHN; auto).
 (* hyp *)
 destruct (eq_nat_dec n0 n);
-simpl. 
+simpl.
   apply closed_w_subst_id;
   replace m with (0+m) by auto;
   apply closed_w_addition; assumption.
   reflexivity.
 (* appl *)
 rewrite IHN1; try rewrite IHN2; auto.
-(* box *)
-destruct w.
-  rewrite IHN; auto.
-  simpl; reflexivity.
-(* letd *)
+(* letdia *)
 destruct w; rewrite IHN1; try rewrite IHN2; auto.
 Qed.
 
 Lemma subst_w_comm:
 forall M w w' w'' n
   (Neq: w'' <> w),
-  {{fwo w'//fwo w''}}({{fwo w//bwo n}}M) = {{fwo w//bwo n}}({{fwo w'//fwo w''}}M).
+  {{fwo w'//fwo w''}}({{fwo w//bwo n}}M) =
+  {{fwo w//bwo n}}({{fwo w'//fwo w''}}M).
 induction M; intros; simpl; try (rewrite IHM; auto).
+(* hyp *)
 reflexivity.
+(* appl *)
 rewrite IHM1; try rewrite IHM2; auto.
 (* get *)
 repeat case_if; subst; auto.
 (* letd *)
-rewrite IHM1; try rewrite IHM2; auto. 
+rewrite IHM1; try rewrite IHM2; auto.
 (* fetch *)
 repeat case_if; subst; auto.
 Qed.
@@ -153,6 +139,7 @@ unfold fresh_world;
 intros; generalize dependent n;
 induction M; intros; simpl in *;
 try (rewrite IHM; auto).
+(* hyp *)
 reflexivity.
 (* appl *)
 apply notin_union in HT;
@@ -163,7 +150,7 @@ repeat case_if; subst; auto.
   subst; apply notin_union in HT; destruct HT;
   elim H; rewrite in_singleton; reflexivity.
 destruct v; auto.
-(* letd *)
+(* letdia *)
 apply notin_union in HT;
 destruct HT;
 rewrite IHM1; try rewrite IHM2; auto.
@@ -181,12 +168,9 @@ forall M w w' n
 intros; generalize dependent n;
 induction M; intros; simpl;
 inversion HT; subst;
-try rewrite IHM; 
-try (rewrite IHM1; try rewrite IHM2); 
-auto.
-(* get *)
-repeat case_if; subst; auto.
-(* fetch *)
+try rewrite IHM;
+try (rewrite IHM1; try rewrite IHM2);
+auto;
 repeat case_if; subst; auto.
 Qed.
 
@@ -196,10 +180,8 @@ forall M n w
   lc_w_n ({{fwo w//bwo n}}M) n.
 intros; generalize dependent n; induction M;
 intros; inversion HT; subst; simpl;
-eauto using lc_w_n.
-repeat case_if; subst; auto.
-constructor; auto.
-repeat case_if; subst; auto.
+eauto using lc_w_n;
+repeat case_if; subst; auto;
 constructor; auto.
 Qed.
 
